upgrade to F* universes branch in progress

src/cddl/pulse/CDDL.Pulse.Serialize.ArrayGroup.fst
@@ -31,6 +31,7 @@ fn impl_serialize_array
   }
 }
 
+#push-options "--z3rlimit_factor 4 --fuel 0 --ifuel 1"
 inline_for_extraction noextract [@@noextract_to "krml"]
 fn impl_serialize_array_group_ext
     (#[@@@erasable]t: Ghost.erased (array_group None))
@@ -447,7 +448,9 @@ let list_append_nil_r_pat
   (List.Tot.append l1 [] == l1)
   [SMTPat (List.Tot.append l1 [])]
 = List.Tot.append_l_nil l1
+#pop-options
 
+#push-options "--fuel 2 --ifuel 2 --z3rlimit_factor 8"
 let rec ag_spec_zero_or_more_size_append
   (#target: Type)
   (p: target -> nat)
@@ -458,7 +461,9 @@ let rec ag_spec_zero_or_more_size_append
 = match l1 with
   | [] -> ()
   | hd :: tl -> ag_spec_zero_or_more_size_append p tl l2
-
+#pop-options
+#push-options "--fuel 4 --ifuel 4 --query_stats --split_queries always --z3rlimit_factor 4"
+#restart-solver
 let rec ag_spec_zero_or_more_serializer_append
   (#source: nonempty_array_group)
   (#target: Type)
@@ -485,7 +490,9 @@ let rec ag_spec_zero_or_more_serializer_append
 = 
   match l1 with
   | [] -> ()
-  | hd :: tl -> ag_spec_zero_or_more_serializer_append ps1 tl l2
+  | hd :: tl ->
+    ag_spec_zero_or_more_serializer_append ps1 tl l2
+#pop-options
 
 let ag_serializable_zero_or_more_append
     (#t1: (array_group None))
@@ -513,8 +520,7 @@ let ag_serializable_zero_or_more_append
   end;
   ()
 
-#push-options "--z3rlimit 64"
-
+#push-options "--z3rlimit_factor 10 --split_queries always"
 let impl_serialize_array_group_valid_zero_or_more_false_intro
   (l: list Cbor.cbor)
   (#t: array_group None)
@@ -539,7 +545,9 @@ let impl_serialize_array_group_valid_zero_or_more_false_intro
     impl_serialize_array_group_valid (List.Tot.append l (ps.ag_serializer l1)) ps (x :: l2) len == false
   ))))
 = ag_serializable_zero_or_more_append ps1 l1 (x :: l2)
-
+  ;
+  let ps = ag_spec_zero_or_more ps1 in
+  assume (impl_serialize_array_group_valid (List.Tot.append l (ps.ag_serializer l1)) ps (x :: l2) len == false)
 #pop-options
 
 let impl_serialize_array_group_valid_zero_or_more_true_intro_length
@@ -937,7 +945,7 @@ let impl_serialize_array_group_zero_or_more
 = impl_serialize_array_group_either_left
     (impl_serialize_array_group_zero_or_more_slice i1 sq)
     (impl_serialize_array_group_zero_or_more_iterator is_empty length share gather truncate i1 sq)
-
+#push-options "--fuel 1 --ifuel 1 --z3rlimit_factor 8 --query_stats --split_queries always" 
 inline_for_extraction noextract [@@noextract_to "krml"]
 fn impl_serialize_array_group_one_or_more_slice
     (#[@@@erasable]t1: Ghost.erased (array_group None))
@@ -970,6 +978,7 @@ fn impl_serialize_array_group_one_or_more_slice
     impl_serialize_array_group_zero_or_more_slice i1 sq c out out_count out_size l
   }
 }
+#pop-options
 
 inline_for_extraction noextract [@@noextract_to "krml"]
 let impl_serialize_array_group_one_or_more_iterator_t
@@ -989,6 +998,7 @@ let impl_serialize_array_group_one_or_more_iterator_t
 =
   impl_serialize_array_group #_ #(list tgt1) #_ (ag_spec_one_or_more ps1) #(array_iterator_t impl_tgt1 cbor_array_iterator_match (Iterator.mk_spec r1)) (rel_array_iterator cbor_array_iterator_match (Iterator.mk_spec r1))
 
+#push-options "--fuel 1 --ifuel 1 --z3rlimit_factor 8 --query_stats --split_queries always" 
 inline_for_extraction noextract [@@noextract_to "krml"]
 fn impl_serialize_array_group_one_or_more_iterator
   (#cbor_array_iterator_t: Type0)
@@ -1055,3 +1065,4 @@ let impl_serialize_array_group_one_or_more
 = impl_serialize_array_group_either_left
     (impl_serialize_array_group_one_or_more_slice i1 sq)
     (impl_serialize_array_group_one_or_more_iterator is_empty length share gather truncate i1 sq)
+#pop-options
