src/cddl/pulse/CDDL.Pulse.Parse.MapGroup.fst
@@ -70,7 +70,8 @@ let impl_zero_copy_map_group
         )
 
 module Util = CBOR.Spec.Util
-
+#push-options "--fuel 1 --ifuel 1 --z3rlimit_factor 8 --query_stats --split_queries always"
+#restart-solver
 inline_for_extraction noextract [@@noextract_to "krml"]
 fn impl_zero_copy_map
   (#ty: Type0)
@@ -1097,7 +1098,9 @@ ensures exists* l .
       as (cbor_map_iterator_match pm contents li)
   };
 }
-
+#pop-options
+#show-options
+#push-options "--z3rlimit_factor 4 --fuel 2 --ifuel 2 --split_queries always --query_stats"
 inline_for_extraction
 fn cddl_map_iterator_next
   (#ty: Type0) (#vmatch: perm -> ty -> cbor -> slprop) (#cbor_map_iterator_t: Type0) (#cbor_map_iterator_match: perm -> cbor_map_iterator_t -> list (cbor & cbor) -> slprop)
@@ -1464,3 +1467,4 @@ fn impl_zero_copy_map_zero_or_more
   Trade.trans _ _ (vmatch p c v);
   res
 }
+#pop-options
