opt/hashes.Makefile
@@ -1,3 +1,3 @@
-FStar_hash := 6cd60f09e1c6cc895b2ea82fc6a91a6af0fcdcb6
+FStar_hash := 9dd6560f885ab3ddad9c752e0810dcad7a4740e7
 karamel_hash := fb36fecb552c9fb202beb38a6c5a732c3f2cd49f
 pulse_hash := 87cb117a6a0eed9ac1c27dbe6ea9572e834284d3
